Add allowed_addrof checks to semantics.

cfrontend/Cexec.v
@@ -374,6 +374,7 @@ Fixpoint step_expr (cp: compartment) (k: kind) (a: expr) (m: mem): reducts expr 
           topred (Lred "red_var_local" (Eloc b Ptrofs.zero Full ty) m)
       | None =>
           do b <- Genv.find_symbol ge x;
+          check Genv.allowed_addrof_b ge cp x;
           topred (Lred "red_var_global" (Eloc b Ptrofs.zero Full ty) m)
       end
   | LV, Ederef r ty =>
@@ -588,7 +589,7 @@ Inductive imm_safe_t (cp: compartment): kind -> expr -> mem -> Prop :=
   | imm_safe_t_loc: forall b ofs ty bf m,
       imm_safe_t cp LV (Eloc b ofs bf ty) m
   | imm_safe_t_lred: forall to C l m l' m',
-      lred ge e l m l' m' ->
+      lred ge e cp l m l' m' ->
       context LV to C ->
       imm_safe_t cp to (C l) m
   | imm_safe_t_rred: forall to C r m t r' m' w',
@@ -624,7 +625,8 @@ Definition invert_expr_prop (cp: compartment) (a: expr) (m: mem) : Prop :=
   | Evar x ty =>
       exists b,
       e!x = Some(b, ty)
-      \/ (e!x = None /\ Genv.find_symbol ge x = Some b)
+      \/ (e!x = None /\ Genv.find_symbol ge x = Some b /\
+            Genv.allowed_addrof ge cp x)
   | Ederef (Eval v ty1) ty =>
       exists b, exists ofs, v = Vptr b ofs
   | Eaddrof (Eloc b ofs bf ty1) ty =>
@@ -685,7 +687,7 @@ Definition invert_expr_prop (cp: compartment) (a: expr) (m: mem) : Prop :=
   end.
 
 Lemma lred_invert:
-  forall cp l m l' m', lred ge e l m l' m' -> invert_expr_prop cp l m.
+  forall cp l m l' m', lred ge e cp l m l' m' -> invert_expr_prop cp l m.
 Proof.
   induction 1; red; auto.
   exists b; auto.
@@ -810,7 +812,7 @@ Local Hint Resolve context_compose contextlist_compose : core.
 
 Definition reduction_ok (cp: compartment) (k: kind) (a: expr) (m: mem) (rd: reduction) : Prop :=
   match k, rd with
-  | LV, Lred _ l' m' => lred ge e a m l' m'
+  | LV, Lred _ l' m' => lred ge e cp a m l' m'
   | RV, Rred _ r' m' t => rred ge cp a m t r' m' /\ exists w', possible_trace w t w'
   | RV, Callred _ fd args tyres t m' => callred ge cp a m fd args tyres t /\ m' = m
   | LV, Stuckred => ~imm_safe_t cp k a m
@@ -1027,7 +1029,12 @@ Proof with (try (apply not_invert_ok; simpl; intro; myinv; intuition congruence;
   destruct (type_eq ty ty')...
   subst. apply topred_ok; auto. apply red_var_local; auto.
   destruct (Genv.find_symbol ge x) as [b|] eqn:?...
-  apply topred_ok; auto. apply red_var_global; auto.
+  destruct Genv.allowed_addrof_b eqn:CHECK...
+  { apply topred_ok; auto. apply red_var_global; auto.
+    now apply Genv.allowed_addrof_b_reflect. }
+  apply not_invert_ok. simpl. rewrite Heqo.
+  intros (? & [?|(_ & _ & CONTRA)]); try easy.
+  apply Genv.allowed_addrof_b_reflect in CONTRA. congruence.
 (* Efield *)
   destruct (is_val a) as [[v ty'] | ] eqn:?.
   rewrite (is_val_inv _ _ _ Heqo).
@@ -1285,14 +1292,17 @@ Qed.
 
 Lemma lred_topred:
   forall cp l1 m1 l2 m2,
-  lred ge e l1 m1 l2 m2 ->
+  lred ge e cp l1 m1 l2 m2 ->
   exists rule, step_expr cp LV l1 m1 = topred (Lred rule l2 m2).
 Proof.
   induction 1; simpl.
 (* var local *)
   rewrite H. rewrite dec_eq_true. econstructor; eauto.
 (* var global *)
-  rewrite H; rewrite H0. econstructor; eauto.
+  rewrite H; rewrite H0.
+  assert (Genv.allowed_addrof_b ge cp x = true) as ->
+    by now rewrite <- Genv.allowed_addrof_b_reflect.
+  econstructor; eauto.
 (* deref *)
   econstructor; eauto.
 (* field struct *)
@@ -1914,7 +1924,7 @@ Proof with (unfold ret; eauto with coqlib).
   inversion H; subst; exploit estep_not_val; eauto; intro NOTVAL.
 (* lred *)
   unfold do_step; rewrite NOTVAL.
-  exploit lred_topred; eauto. instantiate (1 := (comp_of f)). instantiate (1 := w). intros (rule & STEP).
+  exploit lred_topred; eauto. instantiate (1 := w). intros (rule & STEP).
   exists rule. change (TR rule E0 (ExprState f (C a') k e m')) with (expr_final_state f k e (C, Lred rule a' m')).
   apply in_map.
   generalize (step_expr_context e w _ _ _ H1 (comp_of f) a m). unfold reducts_incl.
