cfrontend/Ctyping.v
@@ -1849,8 +1849,8 @@ Proof.
 Qed.
 
 Lemma wt_lred:
-  forall tenv ge e a m a' m',
-  lred ge e a m a' m' -> wt_lvalue ge tenv a -> wt_lvalue ge tenv a'.
+  forall tenv ge e cp a m a' m',
+  lred ge e cp a m a' m' -> wt_lvalue ge tenv a -> wt_lvalue ge tenv a'.
 Proof.
   induction 1; intros WT; constructor.
 Qed.
@@ -1863,8 +1863,8 @@ Proof.
 Qed.
 
 Lemma lred_same_type:
-  forall ge e a m a' m',
-  lred ge e a m a' m' -> typeof a' = typeof a.
+  forall ge e cp a m a' m',
+  lred ge e cp a m a' m' -> typeof a' = typeof a.
 Proof.
   induction 1; auto.
 Qed.
